needs mapply

deps/poulet4/lib/P4cub/Transformations/Lifting/Statementize.v
@@ -10,164 +10,165 @@ Open Scope list_scope.
 
 Section Lift.
   Context {A B : Set}.
-  Variable Lift : nat -> A -> list B * A.
+  Variable Lift : nat -> nat -> A -> list B * A.
   Variable Rename : (nat -> nat) -> A -> A.
+  Variable new : nat.
 
   Fixpoint lift_list
     (up : nat) (l : list A) : list B * list A :=
     match l with
     | []    => ([],[])
     | a :: l =>
-      let '(bs, a') := Lift up a in
-      let '(bss, l') := lift_list (length bs + up) l in
-      (bss ++ bs, Rename (plus $ length bss) a' :: l')
+        let '(bs, a') := Lift new up a in
+        let '(bss, l') := lift_list (length bs + up) l in
+        (bss ++ bs, Rename (plus $ length bss) a' :: l')
     end.
 End Lift.
 
-(** [lift_e up e = (l, e')],
+(** [lift_e new up e = (l, e')],
     where e' is a lifted expression,
     & l is a list of lifted expressions. *)
-Fixpoint lift_e (up : nat) (e : Expr.e) {struct e}
+Fixpoint lift_e (new up : nat) (e : Expr.e) {struct e}
   : list Expr.e * Expr.e :=
   match e with
   | Expr.Bool _
   | Expr.Error _ => ([], e)
   | Expr.Var τ og x => ([], Expr.Var τ og (up + x))
   | Expr.Member t x e
-    => let '(inits, e) := lift_e up e in
+    => let '(inits, e) := lift_e new up e in
       (inits, Expr.Member t x e)
   | Expr.Bit _ _
-  | Expr.Int _ _ => ([e], Expr.Var (t_of_e e) "" 0)
+  | Expr.Int _ _ => ([e], Expr.Var (t_of_e e) "" (up + new))
   | Expr.Slice hi lo eₛ =>
-      let '(inits, eₛ) := lift_e up eₛ in
-      (Expr.Slice hi lo eₛ :: inits, Expr.Var (t_of_e e) "" 0)
+      let '(inits, eₛ) := lift_e new up eₛ in
+      (Expr.Slice hi lo eₛ :: inits, Expr.Var (t_of_e e) "" (up + new))
   | Expr.Cast t e =>
-      let '(inits, e) := lift_e up e in
-      (Expr.Cast t e :: inits, Expr.Var t "" 0)
+      let '(inits, e) := lift_e new up e in
+      (Expr.Cast t e :: inits, Expr.Var t "" (up + new))
   | Expr.Uop t op e =>
-      let '(inits, e) := lift_e up e in
-      (Expr.Uop t op e :: inits, Expr.Var t "" 0)
+      let '(inits, e) := lift_e new up e in
+      (Expr.Uop t op e :: inits, Expr.Var t "" (up + new))
   | Expr.Bop t op lhs rhs => 
-      let '(ll, lhs) := lift_e up lhs in
-      let '(lr, rhs) := lift_e (length ll + up) rhs in
+      let '(ll, lhs) := lift_e new up lhs in
+      let '(lr, rhs) := lift_e new (length ll + up) rhs in
       (Expr.Bop
          t op (rename_e (plus $ length lr) lhs) rhs
-         :: lr ++ ll, Expr.Var t "" 0)
+         :: lr ++ ll, Expr.Var t "" (up + new))
   | Expr.Index t e1 e2 =>
-      let '(l1, e1) := lift_e up e1 in
-      let '(l2, e2) := lift_e (length l1 + up) e2 in
+      let '(l1, e1) := lift_e new up e1 in
+      let '(l2, e2) := lift_e new (length l1 + up) e2 in
       (l2 ++ l1, Expr.Index t (rename_e (plus $ length l2) e1) e2)
   | Expr.Lists l es =>
-      let '(les, es) := lift_list lift_e rename_e up es in
-      (Expr.Lists l es :: les, Expr.Var (t_of_e e) "" 0)
+      let '(les, es) := lift_list lift_e rename_e new up es in
+      (Expr.Lists l es :: les, Expr.Var (t_of_e e) "" (up + new))
   end.
 
 Definition lift_e_list
-  : nat -> list Expr.e -> list Expr.e * list Expr.e :=
+  : nat -> nat -> list Expr.e -> list Expr.e * list Expr.e :=
   lift_list lift_e rename_e.
 
-Definition lift_arg (up : nat) (arg : paramarg Expr.e Expr.e)
+Definition lift_arg (new up : nat) (arg : paramarg Expr.e Expr.e)
   : list Expr.e * paramarg Expr.e Expr.e :=
   match arg with
   | PAIn e =>
-      let '(le, e) := lift_e up e in (le, PAIn e)
+      let '(le, e) := lift_e new up e in (le, PAIn e)
   | PAOut e =>
-      let '(le, e) := lift_e up e in (le, PAOut e)
+      let '(le, e) := lift_e new up e in (le, PAOut e)
   | PAInOut e =>
-      let '(le, e) := lift_e up e in (le, PAInOut e)
+      let '(le, e) := lift_e new up e in (le, PAInOut e)
   end.
 
 Definition lift_args
-  : nat -> Expr.args -> list Expr.e * Expr.args :=
+  : nat -> nat -> Expr.args -> list Expr.e * Expr.args :=
   lift_list lift_arg rename_arg.
 
 (** [unwind_vars [e₁;...;eₙ] s = Stmt.Var eₙ (...(Stmt.Var e₁ s )...)]. *)
 Definition unwind_vars (es : list Expr.e) : Stmt.s -> Stmt.s :=
   List.fold_left (fun b e => Stmt.Var "" (inr e) b) es.
 
-Definition lift_trans (up : nat) (e : Parser.trns)
+Definition lift_trans (new up : nat) (e : Parser.trns)
   : list Expr.e * Parser.trns :=
   match e with
   | Parser.Direct _ => ([],e)
   | Parser.Select e d cases
-    => let '(le,e) := lift_e up e in
+    => let '(le,e) := lift_e new up e in
       (le, Parser.Select e d cases)
   end.
 
-Definition lift_fun_kind (up : nat) (fk : Stmt.fun_kind)
+Definition lift_fun_kind (new up : nat) (fk : Stmt.fun_kind)
   : list Expr.e * Stmt.fun_kind :=
   match fk with
   | Stmt.Funct _ _ None
   | Stmt.Method _ _ _ None => ([],fk)
   | Stmt.Funct f τs (Some e)
-    => let '(le,e) := lift_e up e in (le, Stmt.Funct f τs (Some e))
+    => let '(le,e) := lift_e new up e in (le, Stmt.Funct f τs (Some e))
   | Stmt.Method x m τs (Some e)
-    => let '(le,e) := lift_e up e in (le, Stmt.Method x m τs (Some e))
+    => let '(le,e) := lift_e new up e in (le, Stmt.Method x m τs (Some e))
   | Stmt.Action a es
-    => let '(les,es) := lift_e_list up es in (les, Stmt.Action a es)
+    => let '(les,es) := lift_e_list new up es in (les, Stmt.Action a es)
   end.
 
 Local Open Scope stmt_scope.
 
-Fixpoint lift_s (up : nat) (s : Stmt.s) : Stmt.s :=
+Fixpoint lift_s (new up : nat) (s : Stmt.s) : Stmt.s :=
   match s with
   | Stmt.Skip
   | Stmt.Invoke _
   | Stmt.Exit
   | Stmt.Return None => s
   | Stmt.Return (Some e)
-    => let '(le, e) := lift_e up e in
+    => let '(le, e) := lift_e new up e in
       unwind_vars le $ Stmt.Return $ Some e
   | Stmt.Transition e =>
-      let '(le, e) := lift_trans up e in
+      let '(le, e) := lift_trans new up e in
       unwind_vars le $ Stmt.Transition $ e
   | e₁ `:= e₂
-    => let '(le₁, e₁) := lift_e up e₁ in
-      let '(le₂, e₂) := lift_e (length le₁ + up) e₂ in
+    => let '(le₁, e₁) := lift_e new up e₁ in
+      let '(le₂, e₂) := lift_e new (length le₁ + up) e₂ in
       unwind_vars (le₂ ++ le₁) $ rename_e (plus $ length le₂) e₁ `:= e₂
   | Stmt.Call fk args
-    => let '(lfk,fk) := lift_fun_kind up fk in
-      let '(largs,args) := lift_args (length lfk + up) args in
+    => let '(lfk,fk) := lift_fun_kind new up fk in
+      let '(largs,args) := lift_args new (length lfk + up) args in
       unwind_vars
         (largs ++ lfk) $
         Stmt.Call (rename_fun_kind (plus $ length args) fk) args
   | Stmt.Apply x exts args
-    => let '(inits, args) := lift_args up args in
+    => let '(inits, args) := lift_args new up args in
       unwind_vars inits $ Stmt.Apply x exts args
-  | Stmt.Var og (inl t) s => Stmt.Var og (inl t) (lift_s up s)
+  | Stmt.Var og (inl t) s => Stmt.Var og (inl t) (lift_s (S new) up s)
   | Stmt.Var og (inr e) s =>
-      let '(le,e) := lift_e up e in
+      let '(le,e) := lift_e new up e in
       unwind_vars
         le $ Stmt.Var og (inr e)
-        $ lift_s (length le + up) s
-  | s₁ `; s₂ => lift_s up s₁ `; lift_s up s₂
+        $ lift_s (S new) (length le + up) s
+  | s₁ `; s₂ => lift_s new up s₁ `; lift_s new up s₂
   | If e Then s₁ Else s₂ =>
-      let '(le,e) := lift_e up e in
+      let '(le,e) := lift_e new up e in
       unwind_vars
-        le $ If e Then lift_s (length le + up) s₁
-        Else lift_s (length le + up) s₂
+        le $ If e Then lift_s new (length le + up) s₁
+        Else lift_s new (length le + up) s₂
   end.
 
 Local Close Scope stmt_scope.
 
-Definition lift_control_decl (up : nat) (cd : Control.d) : nat * list Control.d :=
+Definition lift_control_decl (new up : nat) (cd : Control.d) : nat * list Control.d :=
   match cd with
   | Control.Var x (inl t) => (0,[Control.Var x $ inl t])
   | Control.Var x (inr e) =>
-      let '(es, e) := lift_e up e in
+      let '(es, e) := lift_e new up e in
       (List.length es,
         List.map (Control.Var "" ∘ inr) es ++ [Control.Var x $ inr e])
   | Control.Action a cps dps body
-    => (0,[Control.Action a cps dps $ lift_s 0 body])
+    => (0,[Control.Action a cps dps $ lift_s new up body])
   | Control.Table t key acts =>
       let '(es,mks) := List.split key in
       let '(acts,argss) := List.split acts in
-      let '(ees,es) := lift_e_list up es in
+      let '(ees,es) := lift_e_list new up es in
       let '(argsss,argss) :=
         lift_list
           lift_args
           (fun ρ => List.map (rename_arg ρ))
-          (List.length ees + up) argss in
+          new (List.length ees + up) argss in
       (List.length ees + List.length argsss,
         List.map (Control.Var "" ∘ inr) argsss
           ++ List.map (Control.Var "" ∘ inr)
@@ -177,12 +178,12 @@ Definition lift_control_decl (up : nat) (cd : Control.d) : nat * list Control.d 
       
   end.
 
-Fixpoint lift_control_decls (up : nat) (cds : list Control.d) : nat * list Control.d :=
+Fixpoint lift_control_decls (new up : nat) (cds : list Control.d) : nat * list Control.d :=
   match cds with
   | [] => (0, [])
   | d :: ds =>
-      let '(n, d) := lift_control_decl up d in
-      let '(ns, ds) := lift_control_decls (n + up) ds in
+      let '(n, d) := lift_control_decl new up d in
+      let '(ns, ds) := lift_control_decls new (n + up) ds in
       (n + ns, d ++ ds)
   end.
 
@@ -191,16 +192,16 @@ Definition lift_top_decl (td : TopDecl.d) : TopDecl.d :=
   | TopDecl.Instantiate _ _ _ _ _
   | TopDecl.Extern _ _ _ _ _ => td
   | TopDecl.Control c cparams expr_cparams eps params body apply_blk =>
-      let (up, ds) := lift_control_decls 0 body in
+      let (up, ds) := lift_control_decls 0 0 body in
       TopDecl.Control
         c cparams expr_cparams eps params ds
-        $ lift_s up apply_blk  
+        $ lift_s 0 up apply_blk  
   | TopDecl.Parser p cparams expr_cparams eps params start states =>
       TopDecl.Parser
         p cparams expr_cparams eps params
-        (lift_s 0 start) $ map (lift_s 0) states
+        (lift_s 0 0 start) $ map (lift_s 0 0) states
   | TopDecl.Funct f tparams signature body =>
-      TopDecl.Funct f tparams signature $ lift_s 0 body
+      TopDecl.Funct f tparams signature $ lift_s 0 0 body
   end.
 
 Definition lift_program : list TopDecl.d -> list TopDecl.d :=
